theories/Core/Soundness/LogicalRelation/CoreTactics.v
@@ -1,0 +1,8 @@
+From Equations Require Import Equations.
+
+From Mcltt.Core.Soundness Require Import LogicalRelation.Definitions.
+
+Ltac glu_univ_elem_econstructor :=
+  progress simp glu_univ_elem;
+  econstructor;
+  try rewrite <- glu_univ_elem_equation_1 in *.
